Test if relation can be not reflexive

state/FlagBasedEffPoly.fst
@@ -9,23 +9,23 @@ open STLC
 (** for the very general idea, look into experiments/FlagBasedEffPoly.fst **)
 
 type fo_ctx =
-  // fl:erased tflag -> (** we don't have flag yets for ST **) 
   #inv:(lheap -> Type0) -> (** invariant on the heap **)
   #prref: (#a:Type -> #rel:_ -> mref a rel -> Type0) ->
-  #hrel:(FStar.Preorder.preorder lheap) -> (** because of the hrel, we may not need the flag because even if the context uses operations directly, it cannot prove that it preserves the hrel**)
+  #hrel:FStar.Preorder.preorder lheap ->
+ // #hrel:(rel:(lheap -> lheap -> Type0){FStar.Preorder.transitive rel}) -> (** because of the hrel, we may not need the flag because even if the context uses operations directly, it cannot prove that it preserves the hrel**)
   (** ^ if this predicate would be also over heaps, then the contexts needs witness&recall in HO settings **)
   read :  ((#t:typ0) -> r:ref (elab_typ0 t) -> 
             ST (elab_typ0 t) 
               (requires (fun h0 -> inv h0 /\ prref r))
-              (ensures  (fun h0 v h1 -> h0 == h1 /\ sel h1 r == v /\ (elab_typ0_tc t).satisfy_refinement v prref /\ h0 `hrel` h1))) ->
+              (ensures  (fun h0 v h1 -> h0 `hrel` h1 /\ inv h1 /\ (** prref r /\**) (elab_typ0_tc t).satisfy_refinement v prref))) -> // sel h1 r == v /\
   write : ((#t:typ0) -> r:ref (elab_typ0 t) -> v:(elab_typ0 t) -> 
             ST unit
               (requires (fun h0 -> inv h0 /\ prref r /\ (elab_typ0_tc t).satisfy_refinement v prref))
-              (ensures  (fun h0 _ h1 -> inv h1 /\ sel h1 r == v /\ h0 `hrel` h1))) ->
+              (ensures  (fun h0 _ h1 -> h0 `hrel` h1 /\ inv h1 (**/\ prref r /\ (elab_typ0_tc t).satisfy_refinement v prref **)))) -> // /\ sel h1 r == v 
   alloc : ((#t:typ0) -> init:(elab_typ0 t) -> 
             ST (ref (elab_typ0 t)) 
               (requires (fun h0 -> inv h0 /\ (elab_typ0_tc t).satisfy_refinement init prref))
-              (ensures  (fun h0 r h1 -> inv h1 /\ sel h1 r == init /\ prref r /\ h0 `hrel` h1))) ->
+              (ensures  (fun h0 r h1 -> h0 `hrel` h1 /\ inv h1 /\ prref r (** /\ (elab_typ0_tc t).satisfy_refinement init prref **)))) -> // sel h1 r == init /\  
   (** type of the context: *)
   unit -> ST unit (inv) (fun h0 _ h1 -> inv h1 /\ h0 `hrel` h1)
 
@@ -69,6 +69,25 @@ let check_instantiating_the_context (ctx:fo_ctx) =
 
 (** TODO: Can the context easily/automatically work with the pre- and post-conditions? **)
 
+
+open FStar.Tactics
+
+(** CA: this test fails if the relation is not reflexive **)
+val ctx_pure : fo_ctx
+let ctx_pure #inv #_ #hrel my_read my_write my_alloc () : ST unit (inv) (fun h0 _ h1 -> inv h1 /\ h0 `hrel` h1) by (
+  explode ();
+     let bi = nth_binder (-2) in
+     let (_, fl) = destruct_and bi in
+     clear bi;
+     let fl' = instantiate fl (nth_binder (-3)) in
+     clear fl;
+     let fl'' = instantiate fl' (nth_binder (-4)) in
+     clear fl';
+  dump "H"
+)=
+  ()
+  
+  
 val ctx_update_ref_test : fo_ctx
 let ctx_update_ref_test my_read my_write my_alloc () =
   let x = my_alloc 5 in
@@ -80,25 +99,26 @@ type ho_ctx1 = (** only the type of the context is different **)
   #inv:(lheap -> Type0) -> (** invariant on the heap **)
   #prref: (#a:Type -> #rel:_ -> mref a rel -> Type0) ->
   #hrel:(FStar.Preorder.preorder lheap) ->
+  (** ^ if this predicate would be also over heaps, then the contexts needs witness&recall in HO settings **)
   read :  ((#t:typ0) -> r:ref (elab_typ0 t) -> 
             ST (elab_typ0 t) 
               (requires (fun h0 -> inv h0 /\ prref r))
-              (ensures  (fun h0 v h1 -> h0 == h1 /\ sel h1 r == v /\ (elab_typ0_tc t).satisfy_refinement v prref /\ h0 `hrel` h1))) ->
+              (ensures  (fun h0 v h1 -> h0 `hrel` h1 /\ inv h1 /\ (** prref r /\**) (elab_typ0_tc t).satisfy_refinement v prref))) -> // sel h1 r == v /\
   write : ((#t:typ0) -> r:ref (elab_typ0 t) -> v:(elab_typ0 t) -> 
             ST unit
               (requires (fun h0 -> inv h0 /\ prref r /\ (elab_typ0_tc t).satisfy_refinement v prref))
-              (ensures  (fun h0 _ h1 -> inv h1 /\ sel h1 r == v /\ h0 `hrel` h1))) ->
+              (ensures  (fun h0 _ h1 -> h0 `hrel` h1 /\ inv h1 (**/\ prref r /\ (elab_typ0_tc t).satisfy_refinement v prref **)))) -> // /\ sel h1 r == v 
   alloc : ((#t:typ0) -> init:(elab_typ0 t) -> 
             ST (ref (elab_typ0 t)) 
               (requires (fun h0 -> inv h0 /\ (elab_typ0_tc t).satisfy_refinement init prref))
-              (ensures  (fun h0 r h1 -> inv h1 /\ sel h1 r == init /\ prref r /\ h0 `hrel` h1))) ->
+              (ensures  (fun h0 r h1 -> h0 `hrel` h1 /\ inv h1 /\ prref r (** /\ (elab_typ0_tc t).satisfy_refinement init prref **)))) -> // sel h1 r == init /\  
   (** type of the context: *)
   rr:ref (ref int) -> ST (r:ref int -> ST unit (fun h0 -> inv h0 /\ prref r) (fun h0 _ h1 -> inv h1 /\ hrel h0 h1))
     (requires (fun h0 -> inv h0 /\ prref rr))
     (ensures  (fun h0 _ h1 -> inv h1 /\ hrel h0 h1))
 
 val ctx_update_multiple_refs_test : ho_ctx1
-let ctx_update_multiple_refs_test my_read my_write my_alloc x y =
+let ctx_update_multiple_refs_test #inv #prref #hrel my_read my_write my_alloc x y =
   let ix = my_read #(TRef TNat) x in
   my_write #(TRef TNat) x y;
   my_write #TNat y ((my_read #TNat y) + 5);
@@ -108,20 +128,20 @@ let ctx_update_multiple_refs_test my_read my_write my_alloc x y =
 type ho_ctx2 =
   #inv:(lheap -> Type0) -> (** invariant on the heap **)
   #prref: (#a:Type -> #rel:_ -> mref a rel -> Type0) ->
-  #hrel:(FStar.Preorder.preorder lheap) -> (** because of the hrel, we may not need the flag because even if the context uses operations directly, it cannot prove that it preserves the hrel**)
+  #hrel:(rel:(lheap -> lheap -> Type0){FStar.Preorder.transitive rel}) -> (** because of the hrel, we may not need the flag because even if the context uses operations directly, it cannot prove that it preserves the hrel**)
   (** ^ if this predicate would be also over heaps, then the contexts needs witness&recall in HO settings **)
   read :  ((#t:typ0) -> r:ref (elab_typ0 t) -> 
             ST (elab_typ0 t) 
               (requires (fun h0 -> inv h0 /\ prref r))
-              (ensures  (fun h0 v h1 -> h0 == h1 /\ sel h1 r == v /\ (elab_typ0_tc t).satisfy_refinement v prref /\ h0 `hrel` h1))) ->
+              (ensures  (fun h0 v h1 -> inv h1 /\ prref r /\ (elab_typ0_tc t).satisfy_refinement v prref /\ h0 `hrel` h1))) -> // sel h1 r == v /\
   write : ((#t:typ0) -> r:ref (elab_typ0 t) -> v:(elab_typ0 t) -> 
             ST unit
               (requires (fun h0 -> inv h0 /\ prref r /\ (elab_typ0_tc t).satisfy_refinement v prref))
-              (ensures  (fun h0 _ h1 -> inv h1 /\ sel h1 r == v /\ h0 `hrel` h1))) ->
+              (ensures  (fun h0 _ h1 -> inv h1 /\ prref r /\ h0 `hrel` h1 /\ (elab_typ0_tc t).satisfy_refinement v prref))) -> // /\ sel h1 r == v 
   alloc : ((#t:typ0) -> init:(elab_typ0 t) -> 
             ST (ref (elab_typ0 t)) 
               (requires (fun h0 -> inv h0 /\ (elab_typ0_tc t).satisfy_refinement init prref))
-              (ensures  (fun h0 r h1 -> inv h1 /\ sel h1 r == init /\ prref r /\ h0 `hrel` h1))) ->
+              (ensures  (fun h0 r h1 -> inv h1 /\ prref r /\ h0 `hrel` h1 /\ (elab_typ0_tc t).satisfy_refinement init prref))) -> // sel h1 r == init /\  
   (** type of the context: *)
   rr:ref ((ref int) * (ref int)) -> ST (unit -> ST unit (fun h0 -> inv h0) (fun h0 _ h1 -> inv h1 /\ h0 `hrel` h1))
     (requires (fun h0 -> inv h0 /\ prref rr))
